coq/JsPearl.v
@@ -5,18 +5,27 @@ Open Scope Z_scope.
 (* Tiny JavaScript-like expression language. *)
 Inductive expr : Type :=
 | ENum : Z -> expr
-| EAdd : expr -> expr -> expr.
+| EAdd : expr -> expr -> expr
+| ESub : expr -> expr -> expr
+| EMul : expr -> expr -> expr
+| ENeg : expr -> expr.
 
 Fixpoint eval (e : expr) : Z :=
   match e with
   | ENum n => n
   | EAdd a b => eval a + eval b
+  | ESub a b => eval a - eval b
+  | EMul a b => eval a * eval b
+  | ENeg a => - (eval a)
   end.
 
 (* Tiny stack machine target language. *)
 Inductive instr : Type :=
 | IPush : Z -> instr
-| IAdd : instr.
+| IAdd : instr
+| ISub : instr
+| IMul : instr
+| INeg : instr.
 
 Definition stack := list Z.
 Definition program := list instr.
@@ -25,7 +34,13 @@ Definition step (i : instr) (st : stack) : option stack :=
   match i, st with
   | IPush n, _ => Some (n :: st)
   | IAdd, x :: y :: st' => Some ((y + x) :: st')
+  | ISub, x :: y :: st' => Some ((y - x) :: st')
+  | IMul, x :: y :: st' => Some ((y * x) :: st')
+  | INeg, x :: st' => Some ((- x) :: st')
   | IAdd, _ => None
+  | ISub, _ => None
+  | IMul, _ => None
+  | INeg, _ => None
   end.
 
 Fixpoint run (p : program) (st : stack) : option stack :=
@@ -42,6 +57,9 @@ Fixpoint compile (e : expr) : program :=
   match e with
   | ENum n => [IPush n]
   | EAdd a b => compile a ++ compile b ++ [IAdd]
+  | ESub a b => compile a ++ compile b ++ [ISub]
+  | EMul a b => compile a ++ compile b ++ [IMul]
+  | ENeg a => compile a ++ [INeg]
   end.
 
 Lemma run_app : forall p q st st',
@@ -54,15 +72,34 @@ Proof.
     eapply IHp in Hrun. exact Hrun.
 Qed.
 
+Theorem compile_correct_aux : forall e st,
+  run (compile e) st = Some (eval e :: st).
+Proof.
+  induction e as [n|a IHa b IHb|a IHa b IHb|a IHa b IHb|a IHa]; intros st; simpl.
+  - reflexivity.
+  - rewrite run_app with (st' := [eval a]).
+    2: exact (IHa st).
+    rewrite run_app with (st' := [eval b; eval a]).
+    2: exact (IHb (eval a :: st)).
+    simpl. reflexivity.
+  - rewrite run_app with (st' := [eval a]).
+    2: exact (IHa st).
+    rewrite run_app with (st' := [eval b; eval a]).
+    2: exact (IHb (eval a :: st)).
+    simpl. reflexivity.
+  - rewrite run_app with (st' := [eval a]).
+    2: exact (IHa st).
+    rewrite run_app with (st' := [eval b; eval a]).
+    2: exact (IHb (eval a :: st)).
+    simpl. reflexivity.
+  - rewrite run_app with (st' := [eval a]).
+    2: exact (IHa st).
+    simpl. reflexivity.
+Qed.
+
 Theorem compile_correct : forall e,
   run (compile e) [] = Some [eval e].
 Proof.
-  induction e as [n|a IHa b IHb]; simpl.
-  - reflexivity.
-  - rewrite run_app with (st' := [eval a]).
-    2: exact IHa.
-    rewrite run_app with (st' := [eval b; eval a]).
-    2: exact IHb.
-    simpl. reflexivity.
+  intros e. exact (compile_correct_aux e []).
 Qed.
 
